SepLogic/RBT.thy
@@ -1,127 +1,8 @@
 (* Red-black trees. *)
 
 theory RBT
-imports SepAuto Mapping
+imports SepAuto "../Mapping" "../DataStrs/RBT_Base"
 begin
-
-section {* Abstract red-black trees *}
-
-datatype color = R | B
-
-datatype ('a, 'b) rbt =
-  Leaf | Node (lsub: "('a, 'b) rbt") (cl: color) (key: 'a) (val: 'b) (rsub: "('a, 'b) rbt")
-where
-  "cl Leaf = B"
-
-setup {* add_resolve_prfstep @{thm color.distinct(1)} *}
-setup {* add_resolve_prfstep @{thm rbt.distinct(2)} *}
-setup {* fold add_rewrite_rule @{thms rbt.sel} *}
-setup {* add_forward_prfstep (equiv_forward_th (@{thm rbt.simps(1)})) *}
-
-text {* Case checking for trees: first verify the Tip case, then can assume t is
-  in the form Node l c k v r. *}
-
-setup {* add_gen_prfstep ("rbt_case_intro",
-  [WithTerm @{term_pat "?t::(?'a, ?'b) rbt"},
-   Filter (unique_free_filter "t"),
-   CreateCase @{term_pat "(?t::(?'a, ?'b) rbt) = Leaf"}]) *}
-setup {* add_forward_prfstep_cond @{thm rbt.collapse} [with_cond "?rbt \<noteq> Node ?l ?c ?k ?v ?r"] *}
-
-text {* Induction on trees: after checking Tip case, can assume P (lsub t)
-  and P (rsub t) holds when trying to prove P t. *}
-
-theorem rbt_induct': "P Leaf \<Longrightarrow> (\<forall>t. P (lsub t) \<and> P (rsub t) \<longrightarrow> P t) \<Longrightarrow> P t"
-  apply (induction t) apply blast by (metis rbt.sel(1) rbt.sel(6))
-setup {* add_prfstep_induction @{thm rbt_induct'} *}
-
-subsection {* Some trivial lemmas *}
-
-theorem not_R [forward]: "c \<noteq> R \<Longrightarrow> c = B" using color.exhaust by blast
-theorem not_B [forward]: "c \<noteq> B \<Longrightarrow> c = R" using color.exhaust by blast
-theorem red_not_leaf [forward]: "cl t = R \<Longrightarrow> t \<noteq> Leaf" by auto
-
-subsection {* Definition of main functions and invariants *}
-
-fun min_depth :: "('a, 'b) rbt \<Rightarrow> nat" where
-  "min_depth Leaf = 0"
-| "min_depth (Node l c k v r) = min (min_depth l) (min_depth r) + 1"
-
-fun max_depth :: "('a, 'b) rbt \<Rightarrow> nat" where
-  "max_depth Leaf = 0"
-| "max_depth (Node l c k v r) = max (max_depth l) (max_depth r) + 1"
-
-fun black_depth :: "('a, 'b) rbt \<Rightarrow> nat" where
-  "black_depth Leaf = 0"
-| "black_depth (Node l R k v r) = min (black_depth l) (black_depth r)"
-| "black_depth (Node l B k v r) = min (black_depth l) (black_depth r) + 1"
-
-fun cl_inv :: "('a, 'b) rbt \<Rightarrow> bool" where
-  "cl_inv Leaf = True"
-| "cl_inv (Node l R k v r) = (cl_inv l \<and> cl_inv r \<and> cl l = B \<and> cl r = B)"
-| "cl_inv (Node l B k v r) = (cl_inv l \<and> cl_inv r)"
-
-fun bd_inv :: "('a, 'b) rbt \<Rightarrow> bool" where
-  "bd_inv Leaf = True"
-| "bd_inv (Node l c k v r) = (bd_inv l \<and> bd_inv r \<and> black_depth l = black_depth r)"
-
-definition is_rbt :: "('a, 'b) rbt \<Rightarrow> bool" where
-  "is_rbt t = (cl_inv t \<and> bd_inv t)"
-
-setup {* fold add_rewrite_rule (
-  @{thms min_depth.simps} @ @{thms max_depth.simps} @ @{thms black_depth.simps} @
-  @{thms cl_inv.simps} @ @{thms bd_inv.simps} @ [@{thm is_rbt_def}]) *}
-theorem cl_invI: "cl_inv l \<Longrightarrow> cl_inv r \<Longrightarrow> cl_inv (Node l B k v r)" by auto
-setup {* add_forward_prfstep_cond @{thm cl_invI} [with_term "cl_inv (Node ?l B ?k ?v ?r)"] *}
-
-subsection {* Properties of bd_inv *}
-
-theorem bd_inv_elimR [rewrite]:
-  "bd_inv (Node l R k v r) \<Longrightarrow> black_depth (Node l R k v r) = black_depth l" by auto2
-theorem bd_inv_elimB [rewrite]:
-  "bd_inv (Node l B k v r) \<Longrightarrow> black_depth (Node l B k v r) = black_depth l + 1" by auto2
-theorem bd_inv_intro: "black_depth l = black_depth r \<Longrightarrow> bd_inv l \<Longrightarrow> bd_inv r \<Longrightarrow> bd_inv (Node l c k v r)" by auto2
-setup {* add_forward_prfstep_cond @{thm bd_inv_intro} [with_term "Node ?l ?c ?k ?v ?r"] *}
-
-subsection {* is_rbt is recursive *}
-
-theorem is_rbt_rec [forward]: "is_rbt (Node l c k v r) \<Longrightarrow> is_rbt l \<and> is_rbt r"
-  by (tactic {* auto2s_tac @{context} (CASE "c = R") *})
-
-subsection {* Balancedness of is_rbt *}
-
-theorem depth_min: "is_rbt t \<Longrightarrow> black_depth t \<le> min_depth t"
-  by (tactic {* auto2s_tac @{context}
-    (CASE "t = Leaf" THEN
-     CASE "cl t = R" WITH
-        OBTAIN "black_depth t \<le> min (min_depth (lsub t)) (min_depth (rsub t))") *} )
-theorem two_distrib [rewrite]: "(2::nat) * (a + 1) = 2 * a + 2" by simp
-theorem depth_max: "is_rbt t \<Longrightarrow> if cl t = R then max_depth t \<le> 2 * black_depth t + 1
-                                 else max_depth t \<le> 2 * black_depth t"
-  by (tactic {* auto2s_tac @{context}
-    (CASE "t = Leaf" THEN CASE "cl t = R" THEN
-     OBTAIN "max_depth (lsub t) \<le> 2 * black_depth (lsub t) + 1" THEN
-     OBTAIN "max_depth (rsub t) \<le> 2 * black_depth (rsub t) + 1") *} )
-
-setup {* fold add_forward_prfstep [@{thm depth_min}, @{thm depth_max}] *}
-theorem balanced: "is_rbt t \<Longrightarrow> max_depth t \<le> 2 * min_depth t + 1"
-  by (tactic {* auto2s_tac @{context}
-    (OBTAIN "max_depth t \<le> 2 * black_depth t + 1") *})
-setup {* fold del_prfstep_thm [@{thm depth_min}, @{thm depth_max}] *}
-
-subsection {* Definition and basic properties of cl_inv' *}
-
-fun cl_inv' :: "('a, 'b) rbt \<Rightarrow> bool" where
-  "cl_inv' Leaf = True"
-| "cl_inv' (rbt.Node l c k v r) = (cl_inv l \<and> cl_inv r)"
-setup {* fold add_rewrite_rule @{thms cl_inv'.simps} *}
-
-theorem cl_inv_B [forward, backward2]: "rbt.cl t = B \<Longrightarrow> cl_inv' t \<Longrightarrow> cl_inv t" by auto2
-theorem cl_inv_R [forward]:
-  "cl_inv' (rbt.Node l R k v r) \<Longrightarrow> rbt.cl l = B \<Longrightarrow> rbt.cl r = B \<Longrightarrow> cl_inv (rbt.Node l R k v r)" by auto2
-theorem cl_inv_imp [forward]: "cl_inv t \<Longrightarrow> cl_inv' t"
-  by (tactic {* auto2s_tac @{context} (CASE "rbt.cl t = R") *})
-theorem cl_inv'I: "cl_inv l \<Longrightarrow> cl_inv r \<Longrightarrow> cl_inv' (rbt.Node l c k v r)" by auto
-setup {* add_forward_prfstep_cond @{thm cl_inv'I} [with_term "cl_inv' (rbt.Node ?l ?c ?k ?v ?r)"] *}
 
 section {* Tree nodes *}
 
@@ -148,32 +29,38 @@ instance rbt_node :: (heap, heap) heap
   ..
 
 setup {* fold add_rewrite_rule @{thms rbt_node.sel} *}
-theorem rbt_node_constr:
-  "Node l c k v r = Node l' c' k' v' r' \<Longrightarrow> l = l' \<and> c = c' \<and> k = k' \<and> v = v' \<and> r = r'" by simp
-setup {* add_forward_prfstep @{thm rbt_node_constr} *}
+setup {* add_forward_prfstep (equiv_forward_th @{thm rbt_node.simps(1)}) *}
 
-fun btree :: "('a::heap, 'b::heap) rbt \<Rightarrow> ('a, 'b) rbt_node ref option \<Rightarrow> assn" where
+fun btree :: "('a::heap, 'b::heap) pre_rbt \<Rightarrow> ('a, 'b) rbt_node ref option \<Rightarrow> assn" where
   "btree Leaf p = \<up>(p = None)"
-| "btree (rbt.Node lt c k v rt) (Some p) = (\<exists>\<^sub>Alp rp. p \<mapsto>\<^sub>r Node lp c k v rp * btree lt lp * btree rt rp)"
-| "btree (rbt.Node lt c k v rt) None = false"
+| "btree (pre_rbt.Node lt c k v rt) (Some p) = (\<exists>\<^sub>Alp rp. p \<mapsto>\<^sub>r Node lp c k v rp * btree lt lp * btree rt rp)"
+| "btree (pre_rbt.Node lt c k v rt) None = false"
 setup {* fold add_rewrite_rule @{thms btree.simps} *}
 
-lemma btree_split_iff1 [rewrite]: "btree t None = \<up>(t = Leaf)" by auto2
+lemma btree_leaf: "btree Leaf p \<Longrightarrow>\<^sub>A \<up>(p = None)" by auto2
+setup {* add_forward_ent_prfstep_cond @{thm btree_leaf} [K ShadowFirst] *}
 
-lemma btree_split_iff2 [forward_ent]:
-  "btree (rbt.Node lt c k v rt) (Some p) \<Longrightarrow>\<^sub>A (\<exists>\<^sub>Alp rp. p \<mapsto>\<^sub>r Node lp c k v rp * btree lt lp * btree rt rp)" by auto2
+lemma btree_split_iff1: "btree t None \<Longrightarrow>\<^sub>A \<up>(t = Leaf)" by auto2
+setup {* add_forward_ent_prfstep_cond @{thm btree_split_iff1} [K ShadowFirst] *}
+
+lemma btree_split_iff2:
+  "btree (pre_rbt.Node lt c k v rt) (Some p) \<Longrightarrow>\<^sub>A (\<exists>\<^sub>Alp rp. p \<mapsto>\<^sub>r Node lp c k v rp * btree lt lp * btree rt rp)" by auto2
+setup {* add_forward_ent_prfstep_cond @{thm btree_split_iff2} [K ShadowFirst] *}
 
 lemma btree_split_elim:
   "\<exists>lp rp. h \<Turnstile> p \<mapsto>\<^sub>r Node lp c k v rp * Ql lp rp \<Longrightarrow> h \<Turnstile> p \<mapsto>\<^sub>r Node lp c k v rp * Q \<Longrightarrow>
    h \<Turnstile> p \<mapsto>\<^sub>r Node lp c k v rp * Ql lp rp" by auto2
-setup {* add_gen_prfstep ("btree_split_elim", forward_descs @{thm btree_split_elim} @ [ShadowFirst]) *}
+setup {* add_forward_prfstep_cond @{thm btree_split_elim} [K ShadowFirst] *}
 
-lemma btree_is_some: "h \<Turnstile> btree (rbt.Node lt c k v rt) q * Qu \<Longrightarrow> q \<noteq> None" by auto2
-setup {* add_forward_prfstep_cond @{thm btree_is_some} [with_cond "?q \<noteq> None"] *}
+lemma btree_is_some: "h \<Turnstile> btree (pre_rbt.Node lt c k v rt) q * Qu \<Longrightarrow> \<exists>qq. q = Some qq" by auto2
+setup {* add_forward_prfstep_cond @{thm btree_is_some} [with_cond "?q \<noteq> Some ?qq"] *}
 
-lemma btree_constr_ent [forward_ent]:
-  "p \<mapsto>\<^sub>r Node lp c k v rp * btree lt lp * btree rt rp \<Longrightarrow>\<^sub>A btree (rbt.Node lt c k v rt) (Some p)" by auto2
-setup {* del_prfstep_thm @{thm btree.simps(2)} *}
+lemma btree_none: "emp \<Longrightarrow>\<^sub>A btree Leaf None" by auto2
+
+lemma btree_constr_ent:
+  "btree lt lp * btree rt rp * p \<mapsto>\<^sub>r Node lp c k v rp \<Longrightarrow>\<^sub>A btree (pre_rbt.Node lt c k v rt) (Some p)" by auto2
+
+setup {* fold add_entail_matcher [@{thm btree_none}, @{thm btree_constr_ent}] *}
 
 lemma btree_prec [sep_prec_thms]:
   "h \<Turnstile> btree t p * F1 \<Longrightarrow> h \<Turnstile> btree t' p * F2 \<Longrightarrow> t = t'"
@@ -181,11 +68,11 @@ lemma btree_prec [sep_prec_thms]:
     (INDUCT ("t", Arbitraries ["p", "t'", "F1", "F2"]) THEN CASE "t' = Leaf") *})
 
 theorem btree_some [resolve]: "\<not>h \<Turnstile> btree Leaf (Some p) * Ru" by auto2
-theorem btree_none [match_code_pos_emp]: "btree Leaf None = emp" by auto2
 
 lemma rbt_is_not_leaf:
   "h \<Turnstile> btree t (Some p) * Qu \<Longrightarrow> t \<noteq> Leaf" by auto2
-setup {* add_forward_prfstep_cond @{thm rbt_is_not_leaf} [with_cond "?t \<noteq> rbt.Node ?lt ?c ?k ?v ?rt"] *}
+setup {* add_forward_prfstep_cond @{thm rbt_is_not_leaf} [with_cond "?t \<noteq> pre_rbt.Node ?lt ?c ?k ?v ?rt"] *}
+setup {* fold del_prfstep_thm @{thms btree.simps} *}
 
 type_synonym ('a, 'b) btree = "('a, 'b) rbt_node ref option"
 
@@ -197,7 +84,7 @@ definition tree_empty :: "('a, 'b) btree Heap" where
   "tree_empty \<equiv> return None"
 declare tree_empty_def [sep_proc_defs]
 
-lemma tree_empty_rule [next_code_pos]:
+lemma tree_empty_rule [hoare_triple]:
   "<emp> tree_empty <btree Leaf>" by auto2
 
 definition tree_is_empty :: "('a, 'b) btree \<Rightarrow> bool Heap" where
@@ -211,22 +98,22 @@ definition btree_constr :: "('a::heap, 'b::heap) btree \<Rightarrow> color \<Rig
   "btree_constr lp c k v rp = do { p \<leftarrow> ref (Node lp c k v rp); return (Some p) }"
 declare btree_constr_def [sep_proc_defs]
 
-lemma btree_constr_rule [next_code_pos, resolve]:
-  "<btree lt lp * btree rt rp> btree_constr lp c k v rp <btree (rbt.Node lt c k v rt)>" by auto2
+lemma btree_constr_rule [hoare_triple, resolve]:
+  "<btree lt lp * btree rt rp> btree_constr lp c k v rp <btree (pre_rbt.Node lt c k v rt)>" by auto2
 
 partial_function (heap) extract_tree ::
-  "('a::heap, 'b::heap) btree \<Rightarrow> ('a, 'b) rbt Heap" where
+  "('a::heap, 'b::heap) btree \<Rightarrow> ('a, 'b) pre_rbt Heap" where
   "extract_tree p = (case p of
      None \<Rightarrow> return Leaf
    | Some pp \<Rightarrow> do {
       t \<leftarrow> !pp;
       lt \<leftarrow> extract_tree (lsub t);
       rt \<leftarrow> extract_tree (rsub t);
-      return (rbt.Node lt (cl t) (key t) (val t) rt)
+      return (pre_rbt.Node lt (cl t) (key t) (val t) rt)
     })"
 declare extract_tree.simps [sep_proc_defs]
 
-theorem extract_tree_rule [next_code_pos_direct]:
+theorem extract_tree_rule [hoare_triple_direct]:
   "<btree t p> extract_tree p <\<lambda>r. btree t p * \<up>(r = t)>"
   by (tactic {* auto2s_tac @{context} (INDUCT ("t", Arbitraries ["p"])) *})
 
@@ -239,10 +126,10 @@ definition set_color :: "color \<Rightarrow> ('a::heap, 'b::heap) btree \<Righta
     })"
 declare set_color_def [sep_proc_defs]
 
-theorem set_color_rule [next_code_pos]:
-  "<btree (rbt.Node a c x v b) p>
+theorem set_color_rule [hoare_triple]:
+  "<btree (pre_rbt.Node a c x v b) p>
    set_color c' p
-   <\<lambda>r. btree (rbt.Node a c' x v b) p>" by auto2
+   <\<lambda>r. btree (pre_rbt.Node a c' x v b) p>" by auto2
 
 subsection {* Rotation *}
 
@@ -260,25 +147,10 @@ definition btree_rotate_l :: "('a::heap, 'b::heap) btree \<Rightarrow> ('a, 'b) 
           return (rsub t) })})"
 declare btree_rotate_l_def [sep_proc_defs]
 
-lemma btree_rotate_l_rule [next_code_pos]:
-  "<btree (rbt.Node a c1 x v (rbt.Node b c2 y w c)) p>
+lemma btree_rotate_l_rule [hoare_triple]:
+  "<btree (pre_rbt.Node a c1 x v (pre_rbt.Node b c2 y w c)) p>
    btree_rotate_l p
-   <btree (rbt.Node (rbt.Node a c1 x v b) c2 y w c)>" by auto2
-
-definition btree_rotate_l_at_l :: "('a::heap, 'b::heap) btree \<Rightarrow> unit Heap" where
-  "btree_rotate_l_at_l p = (case p of
-    None \<Rightarrow> raise ''rotate_l_at_l''
-  | Some pp \<Rightarrow> do {
-      t \<leftarrow> !pp;
-      p' \<leftarrow> btree_rotate_l (lsub t);
-      pp := Node p' (cl t) (key t) (val t) (rsub t)
-    })"
-declare btree_rotate_l_at_l_def [sep_proc_defs]
-
-lemma btree_rotate_l_at_l_rule [next_code_pos]:
-  "<btree (rbt.Node (rbt.Node a c2 k2 v2 (rbt.Node b c3 k3 v3 c)) c1 k1 v1 d) p>
-   btree_rotate_l_at_l p
-   <\<lambda>_. btree (rbt.Node (rbt.Node (rbt.Node a c2 k2 v2 b) c3 k3 v3 c) c1 k1 v1 d) p>" by auto2
+   <btree (pre_rbt.Node (pre_rbt.Node a c1 x v b) c2 y w c)>" by auto2
 
 definition btree_rotate_r :: "('a::heap, 'b::heap) btree \<Rightarrow> ('a, 'b) btree Heap" where
   "btree_rotate_r p = (case p of
@@ -294,27 +166,12 @@ definition btree_rotate_r :: "('a::heap, 'b::heap) btree \<Rightarrow> ('a, 'b) 
           return (lsub t) })})"
 declare btree_rotate_r_def [sep_proc_defs]
 
-lemma btree_rotate_r_rule [next_code_pos]:
-  "<btree (rbt.Node (rbt.Node a c1 x v b) c2 y w c) p>
+lemma btree_rotate_r_rule [hoare_triple]:
+  "<btree (pre_rbt.Node (pre_rbt.Node a c1 x v b) c2 y w c) p>
    btree_rotate_r p
-   <btree (rbt.Node a c1 x v (rbt.Node b c2 y w c))>" by auto2
+   <btree (pre_rbt.Node a c1 x v (pre_rbt.Node b c2 y w c))>" by auto2
 
-definition btree_rotate_r_at_r :: "('a::heap, 'b::heap) btree \<Rightarrow> unit Heap" where
-  "btree_rotate_r_at_r p = (case p of
-    None \<Rightarrow> raise ''rotate_r_at_r''
-  | Some pp \<Rightarrow> do {
-      t \<leftarrow> !pp;
-      p' \<leftarrow> btree_rotate_r (rsub t);
-      pp := Node (lsub t) (cl t) (key t) (val t) p'
-    })"
-declare btree_rotate_r_at_r_def [sep_proc_defs]
-
-lemma btree_rotate_r_at_r_rule [next_code_pos]:
-  "<btree (rbt.Node a c1 k1 v1 (rbt.Node (rbt.Node b c2 k2 v2 c) c3 k3 v3 d)) p>
-   btree_rotate_r_at_r p
-   <\<lambda>_. btree (rbt.Node a c1 k1 v1 (rbt.Node b c2 k2 v2 (rbt.Node c c3 k3 v3 d))) p>" by auto2
-
-section {* Balancing *}
+section {* Definition of functions *}
 
 definition get_cl :: "('a::heap, 'b::heap) btree \<Rightarrow> color Heap" where
   "get_cl p = (case p of
@@ -325,12 +182,12 @@ definition get_cl :: "('a::heap, 'b::heap) btree \<Rightarrow> color Heap" where
      })"
 declare get_cl_def [sep_proc_defs]
 
-theorem get_cl_heap_preserving [sep_heap_presv_thms, heap_presv_thms]:
+theorem get_cl_heap_preserving [heap_presv_thms]:
   "heap_preserving (get_cl p)"
   by (tactic {* auto2s_tac @{context} (CASE "p = None") *})
 
-theorem get_cl_rule [next_code_pos_direct]:
-  "<btree t p> get_cl p <\<lambda>r. btree t p * \<up>(r = rbt.cl t)>" by auto2
+theorem get_cl_rule [hoare_triple_direct]:
+  "<btree t p> get_cl p <\<lambda>r. btree t p * \<up>(r = pre_rbt.cl t)>" by auto2
 
 definition btree_balanceR :: "('a::heap, 'b::heap) btree \<Rightarrow> ('a, 'b) btree Heap" where
   "btree_balanceR p = (case p of None \<Rightarrow> return None | Some pp \<Rightarrow> do {
@@ -343,7 +200,8 @@ definition btree_balanceR :: "('a::heap, 'b::heap) btree \<Rightarrow> ('a, 'b) 
           cl_lr \<leftarrow> get_cl (lsub rt);
           cl_rr \<leftarrow> get_cl (rsub rt);
           if cl_lr = R then do {
-            btree_rotate_r_at_r p;
+            rp' \<leftarrow> btree_rotate_r (rsub t);
+            pp := Node (lsub t) (cl t) (key t) (val t) rp';
             p' \<leftarrow> btree_rotate_l p;
             t' \<leftarrow> !(the p');
             set_color B (rsub t');
@@ -358,18 +216,6 @@ definition btree_balanceR :: "('a::heap, 'b::heap) btree \<Rightarrow> ('a, 'b) 
      }})"
 declare btree_balanceR_def [sep_proc_defs]
 
-theorem balanceR_bd [next_code_pos]:
-  "<btree t p * \<up>(bd_inv t)>
-   btree_balanceR p
-   <\<lambda>r. \<exists>\<^sub>At'. btree t' r * \<up>(bd_inv t') * \<up>(black_depth t' = black_depth t)>"
-  by auto2
-
-theorem balanceR_cl [next_code_pos]:
-  "<btree (rbt.Node lt B k v rt) p * \<up>(cl_inv lt) * \<up>(cl_inv' rt)>
-   btree_balanceR p
-   <\<lambda>r. \<exists>\<^sub>At'. btree t' r * \<up>(cl_inv t')>"
-  by auto2
-
 definition btree_balance :: "('a::heap, 'b::heap) btree \<Rightarrow> ('a, 'b) btree Heap" where
   "btree_balance p = (case p of None \<Rightarrow> return None | Some pp \<Rightarrow> do {
      t \<leftarrow> !pp;
@@ -381,7 +227,8 @@ definition btree_balance :: "('a::heap, 'b::heap) btree \<Rightarrow> ('a, 'b) b
           cl_rl \<leftarrow> get_cl (rsub lt);
           cl_ll \<leftarrow> get_cl (lsub lt);
           if cl_rl = R then do {
-            btree_rotate_l_at_l p;
+            lp' \<leftarrow> btree_rotate_l (lsub t);
+            pp := Node lp' (cl t) (key t) (val t) (rsub t);
             p' \<leftarrow> btree_rotate_r p;
             t' \<leftarrow> !(the p');
             set_color B (lsub t');
@@ -398,43 +245,6 @@ definition btree_balance :: "('a::heap, 'b::heap) btree \<Rightarrow> ('a, 'b) b
        }
      }})"
 declare btree_balance_def [sep_proc_defs]
-
-theorem balance_bd [next_code_pos]:
-  "<btree t p * \<up>(bd_inv t)>
-   btree_balance p
-   <\<lambda>r. \<exists>\<^sub>At'. btree t' r * \<up>(bd_inv t') * \<up>(black_depth t' = black_depth t)>"
-   by auto2
-
-theorem balance_cl1 [next_code_pos]:
-  "<btree (rbt.Node lt B k v rt) p * \<up>(cl_inv' lt) * \<up>(cl_inv rt)>
-   btree_balance p
-   <\<lambda>r. \<exists>\<^sub>At'. btree t' r * \<up>(cl_inv t')>"
-   by auto2
-
-theorem balance_cl2 [next_code_pos]:
-  "<btree (rbt.Node lt B k v rt) p * \<up>(cl_inv lt) * \<up>(cl_inv' rt)>
-   btree_balance p
-   <\<lambda>r. \<exists>\<^sub>At'. btree t' r * \<up>(cl_inv t')>"
-   by auto2
-
-theorem balanceR_non_leaf [next_code_pos]:
-  "<btree (rbt.Node lt c k v rt) p>
-    btree_balanceR p
-   <\<lambda>r. \<exists>\<^sub>At'. btree t' r * \<up>(t' \<noteq> Leaf)>"
-   by auto2
-
-theorem balance_non_leaf [next_code_pos]:
-  "<btree (rbt.Node lt c k v rt) p>
-    btree_balance p
-   <\<lambda>r. \<exists>\<^sub>At'. btree t' r * \<up>(t' \<noteq> Leaf)>"
-   by auto2
-
-theorem balance_on_R [next_code_pos]:
-  "<btree (rbt.Node lt R k v rt) p>
-   btree_balance p
-   <\<lambda>r. \<exists>\<^sub>At'. btree t' r * \<up>(t' = rbt.Node lt R k v rt)>" by auto2
-
-section {* ins function *}
 
 partial_function (heap) rbt_ins ::
   "'a::{heap,ord} \<Rightarrow> 'b::heap \<Rightarrow> ('a, 'b) btree \<Rightarrow> ('a, 'b) btree Heap" where
@@ -455,25 +265,6 @@ partial_function (heap) rbt_ins ::
          btree_balance p })} )"
 declare rbt_ins.simps [sep_proc_defs]
 
-theorem ins_non_leaf [next_code_pos]:
-  "<btree t p> rbt_ins k v p <\<lambda>r. \<exists>\<^sub>At'. btree t' r * \<up>(t' \<noteq> Leaf)>"
-   by (tactic {* auto2s_tac @{context} (INDUCT ("t", Arbitraries ["p"])) *})
-
-theorem ins_bd [next_code_pos]:
-  "<btree t p * \<up>(bd_inv t)>
-   rbt_ins k v p
-   <\<lambda>r. \<exists>\<^sub>At'. btree t' r * \<up>(bd_inv t') * \<up>(black_depth t' = black_depth t)>"
-   by (tactic {* auto2s_tac @{context} (
-     INDUCT ("t", Arbitraries ["p"]) THEN CASE "rbt.cl t = R") *})
-
-theorem ins_cl [next_code_pos]:
-  "<btree t p * \<up>(cl_inv t)>
-   rbt_ins k v p
-   <\<lambda>r. \<exists>\<^sub>At'. btree t' r * \<up>(if rbt.cl t = B then cl_inv t' else rbt.cl t' = R \<and> cl_inv' t')>"
-   by (tactic {* auto2s_tac @{context} (INDUCT ("t", Arbitraries ["p"])) *})
-
-section {* Insert function *}
-
 definition rbt_insert :: "'a::{heap,ord} \<Rightarrow> 'b::heap \<Rightarrow> ('a, 'b) btree \<Rightarrow> ('a, 'b) btree Heap" where
   "rbt_insert k v p = do {
     p' \<leftarrow> rbt_ins k v p;
@@ -481,178 +272,175 @@ definition rbt_insert :: "'a::{heap,ord} \<Rightarrow> 'b::heap \<Rightarrow> ('
     return p' }"
 declare rbt_insert_def [sep_proc_defs]
 
-theorem insert_is_rbt [next_code_pos]:
+section {* Preservation of black-depth *}
+
+theorem balanceR_bd [hoare_triple]:
+  "<btree t p * \<up>(bd_inv t)>
+   btree_balanceR p
+   <\<lambda>r. \<exists>\<^sub>At'. btree t' r * \<up>(bd_inv t') * \<up>(black_depth t' = black_depth t)>"
+  by auto2
+
+theorem balance_bd [hoare_triple]:
+  "<btree t p * \<up>(bd_inv t)>
+   btree_balance p
+   <\<lambda>r. \<exists>\<^sub>At'. btree t' r * \<up>(bd_inv t') * \<up>(black_depth t' = black_depth t)>"
+  by auto2
+
+theorem ins_bd [hoare_triple]:
+  "<btree t p * \<up>(bd_inv t)>
+   rbt_ins k v p
+   <\<lambda>r. \<exists>\<^sub>At'. btree t' r * \<up>(bd_inv t') * \<up>(black_depth t' = black_depth t)>"
+  by (tactic {* auto2s_tac @{context} (
+    INDUCT ("t", Arbitraries ["p"]) THEN CASE "pre_rbt.cl t = R") *})
+
+setup {* fold del_prfstep_thm [@{thm balanceR_bd}, @{thm balance_bd}] *}
+
+section {* Preservation of cl invariant *}
+
+theorem balanceR_cl [hoare_triple]:
+  "<btree (pre_rbt.Node lt B k v rt) p * \<up>(cl_inv lt) * \<up>(cl_inv' rt)>
+   btree_balanceR p
+   <\<lambda>r. \<exists>\<^sub>At'. btree t' r * \<up>(cl_inv t')>"
+  by auto2
+
+theorem balance_cl1 [hoare_triple]:
+  "<btree (pre_rbt.Node lt B k v rt) p * \<up>(cl_inv' lt) * \<up>(cl_inv rt)>
+   btree_balance p
+   <\<lambda>r. \<exists>\<^sub>At'. btree t' r * \<up>(cl_inv t')>"
+  by auto2
+
+theorem balance_cl2 [hoare_triple]:
+  "<btree (pre_rbt.Node lt B k v rt) p * \<up>(cl_inv lt) * \<up>(cl_inv' rt)>
+   btree_balance p
+   <\<lambda>r. \<exists>\<^sub>At'. btree t' r * \<up>(cl_inv t')>"
+  by auto2
+
+theorem balanceR_non_leaf [hoare_triple]:
+  "<btree (pre_rbt.Node lt c k v rt) p>
+    btree_balanceR p
+   <\<lambda>r. \<exists>\<^sub>At'. btree t' r * \<up>(t' \<noteq> Leaf)>"
+  by auto2
+
+theorem balance_non_leaf [hoare_triple]:
+  "<btree (pre_rbt.Node lt c k v rt) p>
+    btree_balance p
+   <\<lambda>r. \<exists>\<^sub>At'. btree t' r * \<up>(t' \<noteq> Leaf)>"
+  by auto2
+
+theorem balance_on_R [hoare_triple]:
+  "<btree (pre_rbt.Node lt R k v rt) p>
+   btree_balance p
+   <\<lambda>r. \<exists>\<^sub>At'. btree t' r * \<up>(t' = pre_rbt.Node lt R k v rt)>"
+  by auto2
+
+theorem ins_non_leaf [hoare_triple]:
+  "<btree t p> rbt_ins k v p <\<lambda>r. \<exists>\<^sub>At'. btree t' r * \<up>(t' \<noteq> Leaf)>"
+  by (tactic {* auto2s_tac @{context} (INDUCT ("t", Arbitraries ["p"])) *})
+
+theorem ins_cl [hoare_triple]:
+  "<btree t p * \<up>(cl_inv t)>
+   rbt_ins k v p
+   <\<lambda>r. \<exists>\<^sub>At'. btree t' r * \<up>(if pre_rbt.cl t = B then cl_inv t' else pre_rbt.cl t' = R \<and> cl_inv' t')>"
+  by (tactic {* auto2s_tac @{context} (INDUCT ("t", Arbitraries ["p"])) *})
+
+section {* Insert function *}
+
+theorem insert_is_rbt [hoare_triple]:
   "<btree t p * \<up>(is_rbt t)>
    rbt_insert k v p
    <\<lambda>r. \<exists>\<^sub>At'. btree t' r * \<up>(is_rbt t')>" by auto2
 
 (* insert_is_rbt is all we need, so we can clear out bd and cl properties. *)
 setup {* fold del_prfstep_thm [
-  @{thm balanceR_bd}, @{thm balanceR_cl}, @{thm balance_bd},
-  @{thm balance_cl1}, @{thm balance_cl2}, @{thm ins_bd}, @{thm ins_cl}] *}
+  @{thm balanceR_cl}, @{thm balance_cl1}, @{thm balance_cl2}, @{thm ins_bd}, @{thm ins_cl}] *}
 
-section {* Set of keys and mapping associated to an RBT, sortedness on RBT *}
+section {* sortedness on RBT, mapping associated to RBT *}
 
-fun rbt_key_set :: "('a, 'b) rbt \<Rightarrow> 'a set" where
-  "rbt_key_set Leaf = {}"
-| "rbt_key_set (rbt.Node lt c k v rt) = {k} \<union> rbt_key_set lt \<union> rbt_key_set rt"
-setup {* fold add_rewrite_rule @{thms rbt_key_set.simps} *}
-
-fun rbt_sorted :: "('a::linorder, 'b) rbt \<Rightarrow> bool" where
-  "rbt_sorted Leaf = True"
-| "rbt_sorted (rbt.Node lt c k v rt) =
-   ((\<forall>x\<in>rbt_key_set lt. x < k) \<and> (\<forall>x\<in>rbt_key_set rt. k < x) \<and> rbt_sorted lt \<and> rbt_sorted rt)"
-setup {* fold add_rewrite_rule @{thms rbt_sorted.simps} *}
-
-lemma rbt_sorted_on_left [forward]:
-  "rbt_sorted (rbt.Node (rbt.Node a c1 x v b) c2 y w c) \<Longrightarrow> x < y" by auto2 
-
-lemma rbt_sorted_on_right [forward]:
-  "rbt_sorted (rbt.Node a c1 x v (rbt.Node b c2 y w c)) \<Longrightarrow> x < y" by auto2
-
-fun tree_map :: "('a::linorder, 'b) rbt \<Rightarrow> ('a, 'b) map" where
-  "tree_map Leaf = Map (\<lambda>x. None)"
-| "tree_map (rbt.Node lt c k v rt) = binary_map k v (tree_map lt) (tree_map rt)"
-setup {* fold add_rewrite_rule @{thms tree_map.simps} *}
-
-(* Sortedness and preservation of set of keys is best proved by
-   introducing in-order traversal. *)
-fun rbt_in_traverse :: "('a, 'b) rbt \<Rightarrow> 'a list" where
-  "rbt_in_traverse Leaf = []"
-| "rbt_in_traverse (rbt.Node lt c k v rt) = (rbt_in_traverse lt) @ [k] @ (rbt_in_traverse rt)"
-setup {* fold add_rewrite_rule @{thms rbt_in_traverse.simps} *}
-
-theorem rbt_in_traverse_non_empty:
-  "rbt_in_traverse (rbt.Node lt c k v rt) \<noteq> []" by auto2
-
-theorem inorder_preserve_set [rewrite_bidir]:
-  "set (rbt_in_traverse t) = rbt_key_set t" by auto2
-
-fun strict_sorted :: "'a::linorder list \<Rightarrow> bool" where
-  "strict_sorted [] = True"
-| "strict_sorted (x # ys) = ((\<forall>y\<in>set ys. x < y) \<and> strict_sorted ys)"
-setup {* fold add_rewrite_rule @{thms strict_sorted.simps} *}
-
-theorem strict_sorted_single [resolve]: "strict_sorted [x]" by auto2
-setup {* del_prfstep_thm @{thm strict_sorted.simps(2)} #>
-  add_rewrite_rule_cond @{thm strict_sorted.simps(2)} [with_cond "?ys \<noteq> []"] *}
-
-theorem strict_sorted_append [rewrite]:
-  "strict_sorted (xs @ ys) =
-    ((\<forall>x y. x \<in> set xs \<longrightarrow> y \<in> set ys \<longrightarrow> x < y) \<and> strict_sorted xs \<and> strict_sorted ys)"
-  by (tactic {* auto2s_tac @{context} (INDUCT ("xs", [])) *})
-
-theorem inorder_sorted [rewrite_bidir]:
-  "strict_sorted (rbt_in_traverse t) = rbt_sorted t" by auto2
-setup {* del_prfstep_thm @{thm strict_sorted_append} *}
-
-theorem balanceR_in_traverse [next_code_pos]:
+theorem balanceR_in_traverse_pairs [hoare_triple]:
   "<btree t p>
    btree_balanceR p
-   <\<lambda>r. \<exists>\<^sub>At'. btree t' r * \<up>(rbt_in_traverse t' = rbt_in_traverse t)>"
+   <\<lambda>r. \<exists>\<^sub>At'. btree t' r * \<up>(rbt_in_traverse_pairs t' = rbt_in_traverse_pairs t)>"
   by auto2
 
-theorem balance_in_traverse [next_code_pos]:
+theorem balance_in_traverse_pairs [hoare_triple]:
   "<btree t p>
    btree_balance p
-   <\<lambda>r. \<exists>\<^sub>At'. btree t' r * \<up>(rbt_in_traverse t' = rbt_in_traverse t)>"
+   <\<lambda>r. \<exists>\<^sub>At'. btree t' r * \<up>(rbt_in_traverse_pairs t' = rbt_in_traverse_pairs t)>"
   by auto2
 
 declare btree_balance_def [sep_proc_defs del]
-theorem balance_sorted [next_code_pos]:
-  "<btree t p * \<up>(rbt_sorted t)>
-   btree_balance p
-   <\<lambda>r. \<exists>\<^sub>At'. btree t' r * \<up>(rbt_sorted t')>"
-  by auto2
 
-theorem balance_key_set [next_code_pos]:
-  "<btree t p>
-   btree_balance p
-   <\<lambda>r. \<exists>\<^sub>At'. btree t' r * \<up>(rbt_key_set t' = rbt_key_set t)>"
-  by auto2
-declare btree_balance_def [sep_proc_defs]
-
-theorem ins_key_set [next_code_pos]:
-  "<btree t p>
-   rbt_ins k v p
-   <\<lambda>r. \<exists>\<^sub>At'. btree t' r * \<up>(rbt_key_set t' = {k} \<union> rbt_key_set t)>"
-  by (tactic {* auto2s_tac @{context} (INDUCT ("t", Arbitraries ["p"])) *})
-
-theorem ins_sorted [next_code_pos]:
+theorem ins_inorder_pairs [hoare_triple]:
   "<btree t p * \<up>(rbt_sorted t)>
    rbt_ins k v p
-   <\<lambda>r. \<exists>\<^sub>At'. btree t' r * \<up>(rbt_sorted t')>"
+   <\<lambda>r. \<exists>\<^sub>At'. btree t' r * \<up>(rbt_in_traverse_pairs t' = ordered_insert_pairs k v (rbt_in_traverse_pairs t))>"
   by (tactic {* auto2s_tac @{context} (INDUCT ("t", Arbitraries ["p"])) *})
 
-theorem insert_key_set [next_code_pos]:
-  "<btree t p>
-   rbt_insert k v p
-   <\<lambda>r. \<exists>\<^sub>At'. btree t' r * \<up>(rbt_key_set t' = {k} \<union> rbt_key_set t)>"
-  by auto2
-
-theorem insert_sorted [next_code_pos]:
+theorem insert_inorder_pairs [hoare_triple]:
   "<btree t p * \<up>(rbt_sorted t)>
    rbt_insert k v p
-   <\<lambda>r. \<exists>\<^sub>At'. btree t' r * \<up>(rbt_sorted t')>"
+   <\<lambda>r. \<exists>\<^sub>At'. btree t' r * \<up>(rbt_in_traverse_pairs t' = ordered_insert_pairs k v (rbt_in_traverse_pairs t))>"
   by auto2
 
-(* Finally, we prove effect of operations on mapping *)
+declare rbt_insert_def [sep_proc_defs del]
 
-lemma btree_rotate_preserves_map:
-  "x < y \<Longrightarrow> tree_map (rbt.Node a c1 x v (rbt.Node b c2 y w c)) =
-   tree_map (rbt.Node (rbt.Node a c3 x v b) c4 y w c)" by auto2
-setup {* add_forward_prfstep_cond @{thm btree_rotate_preserves_map}
-  [with_term "rbt.Node ?a ?c1.0 ?x ?v (rbt.Node ?b ?c2.0 ?y ?w ?c)",
-   with_term "rbt.Node (rbt.Node ?a ?c3.0 ?x ?v ?b) ?c4.0 ?y ?w ?c"] *}
-
-theorem balanceR_map [next_code_pos]:
-  "<btree t p * \<up>(rbt_sorted t)>
-   btree_balanceR p
-   <\<lambda>r. \<exists>\<^sub>At'. btree t' r * \<up>(tree_map t' = tree_map t)>"
-  by auto2
-
-theorem balance_map [next_code_pos, code_pos_create_case]:
-  "<btree t p * \<up>(rbt_sorted t)>
-   btree_balance p
-   <\<lambda>r. \<exists>\<^sub>At'. btree t' r * \<up>(tree_map t' = tree_map t)>"
-  by auto2
-
-theorem ins_map [next_code_pos]:
-  "<btree t p * \<up>(rbt_sorted t)>
-   rbt_ins k v p
-   <\<lambda>r. \<exists>\<^sub>At'. btree t' r * \<up>(tree_map t' = (tree_map t) {k \<rightarrow> v})>"
-  by (tactic {* auto2s_tac @{context} (INDUCT ("t", Arbitraries ["p"])) *})
-
-theorem insert_map [next_code_pos]:
+theorem insert_sorted [hoare_triple]:
   "<btree t p * \<up>(rbt_sorted t)>
    rbt_insert k v p
-   <\<lambda>r. \<exists>\<^sub>At'. btree t' r * \<up>(tree_map t' = (tree_map t) {k \<rightarrow> v})>"
-  by auto2
+   <\<lambda>r. \<exists>\<^sub>At'. btree t' r * \<up>(rbt_sorted t')>" by auto2
+
+theorem insert_tree_map [hoare_triple]:
+  "<btree t p * \<up>(rbt_sorted t)>
+   rbt_insert k v p
+   <\<lambda>r. \<exists>\<^sub>At'. btree t' r * \<up>(rbt_map t' = (rbt_map t) {k \<rightarrow> v})>" by auto2
+
+section {* Search function *}
+
+partial_function (heap) rbt_search ::
+  "'a::{heap,linorder} \<Rightarrow> ('a, 'b::heap) btree \<Rightarrow> 'b option Heap" where
+  "rbt_search x b = (case b of
+     None \<Rightarrow> return None
+   | Some p \<Rightarrow> do {
+      t \<leftarrow> !p;
+      (if x = key t then return (Some (val t))
+       else if x < key t then rbt_search x (lsub t)
+       else rbt_search x (rsub t)) })"
+declare rbt_search.simps [sep_proc_defs]
+
+lemma btree_search_correct [hoare_triple]:
+  "<btree t b * \<up>(rbt_sorted t)>
+   rbt_search x b
+   <\<lambda>r. btree t b * \<up>(r = (rbt_map t)\<langle>x\<rangle>)>"
+  by (tactic {* auto2s_tac @{context} (INDUCT ("t", Arbitraries ["b"])) *})
+declare rbt_search.simps [sep_proc_defs del]
 
 section {* Outer interface *}
 
-definition rbt_set :: "'a set \<Rightarrow> ('a::{heap,linorder}, 'b::heap) rbt_node ref option \<Rightarrow> assn" where
-  "rbt_set S p = (\<exists>\<^sub>At. btree t p * \<up>(is_rbt t) * \<up>(rbt_sorted t) * \<up>(S = rbt_key_set t))"
-setup {* add_rewrite_rule @{thm rbt_set_def} *}
+definition rbt_set_assn :: "'a set \<Rightarrow> ('a::{heap,linorder}, 'b::heap) rbt_node ref option \<Rightarrow> assn" where
+  "rbt_set_assn S p = (\<exists>\<^sub>At. btree t p * \<up>(is_rbt t) * \<up>(rbt_sorted t) * \<up>(S = rbt_set t))"
+setup {* add_rewrite_rule @{thm rbt_set_assn_def} *}
 
-definition rbt_map :: "('a, 'b) map \<Rightarrow> ('a::{heap,linorder}, 'b::heap) rbt_node ref option \<Rightarrow> assn" where
-  "rbt_map M p = (\<exists>\<^sub>At. btree t p * \<up>(is_rbt t) * \<up>(rbt_sorted t) * \<up>(M = tree_map t))"
-setup {* add_rewrite_rule @{thm rbt_map_def} *}
+definition rbt_map_assn :: "('a, 'b) map \<Rightarrow> ('a::{heap,linorder}, 'b::heap) rbt_node ref option \<Rightarrow> assn" where
+  "rbt_map_assn M p = (\<exists>\<^sub>At. btree t p * \<up>(is_rbt t) * \<up>(rbt_sorted t) * \<up>(M = rbt_map t))"
+setup {* add_rewrite_rule @{thm rbt_map_assn_def} *}
 
 declare tree_empty_def [sep_proc_defs del]
 
 lemma rbt_empty_rule1:
-  "<emp> tree_empty <rbt_set {}>" by auto2
+  "<emp> tree_empty <rbt_set_assn {}>" by auto2
 
 lemma rbt_empty_rule2:
-  "<emp> tree_empty <rbt_map empty_map>" by auto2
+  "<emp> tree_empty <rbt_map_assn empty_map>" by auto2
 
 declare rbt_insert_def [sep_proc_defs del]
 
 lemma rbt_insert_rule1:
-  "<rbt_set S b> rbt_insert k v b <rbt_set ({k} \<union> S)>" by auto2
+  "<rbt_set_assn S b> rbt_insert k v b <rbt_set_assn ({k} \<union> S)>" by auto2
 
 lemma rbt_insert_rule2:
-  "<rbt_map M b> rbt_insert k v b <rbt_map (M {k \<rightarrow> v})>" by auto2
+  "<rbt_map_assn M b> rbt_insert k v b <rbt_map_assn (M {k \<rightarrow> v})>" by auto2
+
+lemma rbt_search:
+  "<rbt_map_assn M b> rbt_search x b <\<lambda>r. rbt_map_assn M b * \<up>(r = M\<langle>x\<rangle>)>" by auto2
 
 end
