Analysis/Equiv_Rel_Thms.thy
@@ -1,8 +1,0 @@
-theory Equiv_Rel_Thms
-imports "../Auto2"
-begin
-
-setup {* add_rewrite_rule @{thm symp_def} *}
-setup {* add_rewrite_rule @{thm transp_def} *}
-
-end
