SepLogic/DynamicArray.thy
@@ -48,7 +48,7 @@ definition dyn_array_new :: "'a \<Rightarrow> 'a::heap dynamic_array Heap" where
    }"
 declare dyn_array_new_def [sep_proc_defs]
 
-theorem dyn_array_new_rule [next_code_pos]:
+theorem dyn_array_new_rule [hoare_triple]:
   "<emp> dyn_array_new x <dyn_array []>" by auto2
 
 fun array_copy :: "'a::heap array \<Rightarrow> nat \<Rightarrow> 'a array \<Rightarrow> nat \<Rightarrow> nat \<Rightarrow> unit Heap" where
@@ -61,7 +61,7 @@ fun array_copy :: "'a::heap array \<Rightarrow> nat \<Rightarrow> 'a array \<Rig
      })"
 declare array_copy.simps [sep_proc_defs]
 
-theorem array_copy_rule [next_code_pos, code_pos_create_case]:
+theorem array_copy_rule [hoare_triple, hoare_create_case]:
   "<src \<mapsto>\<^sub>a lsrc * dst \<mapsto>\<^sub>a ldst * \<up>(si + len \<le> length lsrc) * \<up>(di + len \<le> length ldst)>
     array_copy src si dst di len
    <\<lambda>_. src \<mapsto>\<^sub>a lsrc * dst \<mapsto>\<^sub>a list_update_range ldst di (take len (drop si lsrc))>"
@@ -78,7 +78,7 @@ definition ensure_length :: "nat \<Rightarrow> 'a::heap dynamic_array \<Rightarr
       } else return d)"
 declare ensure_length_def [sep_proc_defs]
 
-theorem ensure_length_rule [next_code_pos]:
+theorem ensure_length_rule [hoare_triple]:
   "<dyn_array xs p> ensure_length nl p <\<lambda>r. dyn_array xs r * \<up>(amax r \<ge> nl)>\<^sub>t" by auto2
 
 definition push_array :: "'a \<Rightarrow> 'a::heap dynamic_array \<Rightarrow> 'a dynamic_array Heap" where
@@ -89,7 +89,7 @@ definition push_array :: "'a \<Rightarrow> 'a::heap dynamic_array \<Rightarrow> 
       return (Dyn_Array (alen p + 1) (amax p) (defv p) (aref p)) })"
 declare push_array_def [sep_proc_defs]
 
-theorem push_array_rule [next_code_pos]:
+theorem push_array_rule [hoare_triple]:
   "<dyn_array xs p> push_array x p <\<lambda>r. dyn_array (xs @ [x]) r>\<^sub>t" by auto2
 
 definition pop_array :: "'a::heap dynamic_array \<Rightarrow> ('a \<times> 'a dynamic_array) Heap" where
@@ -100,19 +100,19 @@ definition pop_array :: "'a::heap dynamic_array \<Rightarrow> ('a \<times> 'a dy
     })"
 declare pop_array_def [sep_proc_defs]
 
-theorem pop_array_rule [next_code_pos]:
+theorem pop_array_rule [hoare_triple]:
   "<dyn_array xs p * \<up>(length xs > 0)>
    pop_array p
    <\<lambda>(x, r). dyn_array (butlast xs) r * \<up>(x = last xs)>" by auto2
 
-theorem pop_array_heap_preserving [sep_heap_presv_thms, heap_presv_thms]:
+theorem pop_array_heap_preserving [heap_presv_thms]:
   "heap_preserving (pop_array d)" by auto2
 
 definition array_upd :: "nat \<Rightarrow> 'a \<Rightarrow> 'a::heap dynamic_array \<Rightarrow> unit Heap" where
   "array_upd i x d = do { Array.upd i x (aref d); return () }"
 declare array_upd_def [sep_proc_defs]
 
-theorem array_upd_rule [next_code_pos, code_pos_create_case]:
+theorem array_upd_rule [hoare_triple, hoare_create_case]:
   "<dyn_array l p * \<up>(i < length l)>
    array_upd i x p
    <\<lambda>_. dyn_array (list_update l i x) p>" by auto2
@@ -121,24 +121,24 @@ definition array_nth :: "'a::heap dynamic_array \<Rightarrow> nat \<Rightarrow> 
   "array_nth d i = Array.nth (aref d) i"
 declare array_nth_def [sep_proc_defs]
 
-theorem array_nth_rule [next_code_pos, code_pos_create_case]:
+theorem array_nth_rule [hoare_triple, hoare_create_case]:
   "<dyn_array xs p * \<up>(i < length xs)>
    array_nth p i
    <\<lambda>r. dyn_array xs p * \<up>(r = xs ! i)>" by auto2
 
-theorem array_nth_heap_preserving [sep_heap_presv_thms, heap_presv_thms]:
+theorem array_nth_heap_preserving [heap_presv_thms]:
   "heap_preserving (array_nth d i)" by auto2
 
 definition array_length :: "'a dynamic_array \<Rightarrow> nat Heap" where
   "array_length d = return (alen d)"
 declare array_length_def [sep_proc_defs]
 
-theorem array_length_rule [next_code_pos_direct]:
+theorem array_length_rule [hoare_triple_direct]:
   "<dyn_array xs p>
    array_length p
    <\<lambda>r. dyn_array xs p * \<up>(r = length xs)>" by auto2
 
-theorem array_length_heap_preserving [sep_heap_presv_thms, heap_presv_thms]:
+theorem array_length_heap_preserving [heap_presv_thms]:
   "heap_preserving (array_length d)" by auto2
 
 definition array_swap :: "'a::heap dynamic_array \<Rightarrow> nat \<Rightarrow> nat \<Rightarrow> unit Heap" where
@@ -151,7 +151,7 @@ definition array_swap :: "'a::heap dynamic_array \<Rightarrow> nat \<Rightarrow>
    }"
 declare array_swap_def [sep_proc_defs]
 
-theorem array_swap_rule [next_code_pos, code_pos_create_case]:
+theorem array_swap_rule [hoare_triple, hoare_create_case]:
   "<dyn_array xs p * \<up>(i < length xs) * \<up>(j < length xs)>
    array_swap p i j
    <\<lambda>_. dyn_array (list_swap xs i j) p>" by auto2
