SepLogic/SepAuto.thy
@@ -7,14 +7,34 @@ subsection {* Assertions *}
 theorem mod_ex_distrib_star [rewrite]: "(h \<Turnstile> (\<exists>\<^sub>Ax. P x) * Q) = (h \<Turnstile> (\<exists>\<^sub>Ax. P x * Q))"
   by (simp add: ex_distrib_star)
 
-theorem ex_distrib_star_l:
-  "(\<exists>\<^sub>Ax. (Q * P x)) = (Q * (\<exists>\<^sub>Ax. P x))" by auto2
+theorem ex_distrib_star_l:  "(\<exists>\<^sub>Ax. (Q * P x)) = (Q * (\<exists>\<^sub>Ax. P x))" by auto2
+
+theorem pure_conj:  "\<up>(P \<and> Q) = \<up>P * \<up>Q" by auto2
 
 theorem pure_assn_eq_same [resolve]: "P * \<up>(x = x) = P" by auto2
 theorem mod_false' [resolve]: "\<not> (h \<Turnstile> false * Ru)" by auto2
 theorem mod_star_true [resolve]: "h \<Turnstile> P * Ru \<Longrightarrow> h \<Turnstile> P * true"
   by (tactic {* auto2s_tac @{context} (OBTAIN "Ru \<Longrightarrow>\<^sub>A true") *})
 theorem mod_star_true' [resolve]: "h \<Turnstile> R \<Longrightarrow> h \<Turnstile> true" by auto2
+theorem mod_star_true2 [backward2]: "h \<Turnstile> P x * R \<Longrightarrow> Q x \<Longrightarrow> \<exists>x. (h \<Turnstile> P x * true) \<and> Q x"
+  by (tactic {* auto2s_tac @{context} (OBTAIN "h \<Turnstile> P x * true") *})
+
+subsection {* Entailment *}
+
+theorem entails_triv: "A \<Longrightarrow>\<^sub>A A" by auto2
+theorem entail_trans: "A \<Longrightarrow>\<^sub>A B \<Longrightarrow> B \<Longrightarrow>\<^sub>A C \<Longrightarrow> A \<Longrightarrow>\<^sub>A C" by auto2
+theorem entail_trans2: "A \<Longrightarrow>\<^sub>A D * B \<Longrightarrow> B \<Longrightarrow>\<^sub>A C \<Longrightarrow> A \<Longrightarrow>\<^sub>A D * C"
+  by (simp add: assn_times_comm entailsD' entails_def)
+theorem entail_trans3: "A \<Longrightarrow>\<^sub>A B * C \<Longrightarrow> B \<Longrightarrow>\<^sub>A D \<Longrightarrow> A \<Longrightarrow>\<^sub>A D * C"
+  by (simp add: entailsD' entails_def)
+
+theorem mod_array_eq [backward1]: "xs = xs' \<Longrightarrow> h \<Turnstile> p \<mapsto>\<^sub>a xs \<Longrightarrow> h \<Turnstile> p \<mapsto>\<^sub>a xs'" by simp
+
+subsection {* outer_remains for Arrays *}
+
+definition outer_remains :: "'a list \<Rightarrow> 'a list \<Rightarrow> nat \<Rightarrow> nat \<Rightarrow> bool" where
+  "outer_remains xs xs' l r = (length xs = length xs' \<and> (\<forall>i. i < l \<or> r < i \<longrightarrow> xs ! i = xs' ! i))"
+setup {* add_rewrite_rule @{thm outer_remains_def} *}
 
 subsection {* Clear unused proofsteps *}
 
@@ -28,45 +48,55 @@ subsection {* Definition of procedures *}
 
 named_theorems sep_proc_defs "Seplogic: definitions of procedures"
 named_theorems sep_prec_thms "Seplogic: precision theorems"
+(* Note adding to sep_heap_presv_thms is taken care of by heap_presv_thms attribute. *)
 named_theorems sep_heap_presv_thms "Seplogic: heap preservation theorems"
 
 declare ref_prec [sep_prec_thms]
 declare array_ref_prec [sep_prec_thms]
 
 (* ASCII abbreviations for ML files. *)
-abbreviation ex_assn_ascii :: "('a \<Rightarrow> assn) \<Rightarrow> assn" (binder "EXA" 11)
+abbreviation (input) ex_assn_ascii :: "('a \<Rightarrow> assn) \<Rightarrow> assn" (binder "EXA" 11)
   where "ex_assn_ascii \<equiv> ex_assn"
 
-abbreviation models_ascii :: "pheap \<Rightarrow> assn \<Rightarrow> bool" (infix "|=" 50)
+abbreviation (input) models_ascii :: "pheap \<Rightarrow> assn \<Rightarrow> bool" (infix "|=" 50)
   where "h |= P \<equiv> h \<Turnstile> P"
 
 ML_file "sep_steps.ML"
 ML_file "sep_steps_test.ML"
+ML_file "assn_matcher.ML"
+ML_file "sep_induct.ML"
 
+setup {* Logic_ProofSteps.add_priority_term @{const_name models} *}
 attribute_setup heap_presv_thms = {* setup_attrib Sep_Logic.add_heap_preserving_thm_gnrc *}
 attribute_setup forward_ent = {* setup_attrib Sep_Logic.add_forward_ent_prfstep_gnrc *}
-attribute_setup match_code_pos_emp = {* setup_attrib Sep_Logic.add_match_code_pos_emp_prfstep_gnrc *}
-attribute_setup code_pos_create_case = {* setup_attrib Sep_Logic.add_match_code_pos_create_case_gnrc *}
-attribute_setup next_code_pos = {* setup_attrib Sep_Logic.add_next_code_pos_prfstep_gnrc *}
-attribute_setup next_code_pos_direct = {* setup_attrib Sep_Logic.add_next_code_pos_direct_prfstep_gnrc *}
+attribute_setup hoare_create_case = {* setup_attrib Sep_Logic.add_match_hoare_create_case_gnrc *}
+attribute_setup hoare_triple = {* setup_attrib Sep_Logic.add_hoare_triple_prfstep_gnrc *}
+attribute_setup hoare_triple_direct = {* setup_attrib Sep_Logic.add_hoare_triple_direct_prfstep_gnrc *}
 
-theorem basic_heap_preserving_thms [sep_heap_presv_thms, heap_presv_thms]:
+theorem basic_heap_preserving_thms [heap_presv_thms]:
   "heap_preserving (!p)"
   "heap_preserving (return x)"
   "heap_preserving (Array.nth a i)"
   "heap_preserving (Array.len a)"
 by (smt effect_lookupE effect_returnE effect_nthE effect_lengthE heap_preserving_def)+
 
-setup {* add_next_code_pos_direct_prfstep @{thm return_rule} *}
-setup {* add_next_code_pos_prfstep @{thm ref_rule} *}
-setup {* add_next_code_pos_direct_prfstep @{thm lookup_rule} *}
-setup {* add_next_code_pos_prfstep @{thm update_rule} *}
-setup {* add_next_code_pos_prfstep @{thm new_rule} *}
-setup {* add_next_code_pos_prfstep @{thm nth_rule} *}
-declare nth_rule [code_pos_create_case]
-setup {* add_next_code_pos_prfstep @{thm upd_rule} *}
-declare upd_rule [code_pos_create_case]
-setup {* add_next_code_pos_direct_prfstep @{thm length_rule} *}
+theorem heap_preserve_comment [heap_presv_thms]: "heap_preserving (comment P)"
+  by (simp add: comment_def effect_def heap_preserving_def)
+
+theorem heap_preserve_assert [heap_presv_thms]: "heap_preserving (assert P x)"
+  using effect_assertE heap_preserving_def by fastforce
+
+declare comment_rule [hoare_triple]
+declare comment_rule2 [hoare_triple, hoare_create_case]
+declare assert_rule [hoare_triple, hoare_create_case]
+declare return_rule [hoare_triple_direct]
+declare ref_rule [hoare_triple_direct]
+declare lookup_rule [hoare_triple_direct]
+declare update_rule [hoare_triple]
+declare new_rule [hoare_triple_direct]
+declare nth_rule [hoare_triple, hoare_create_case]
+declare upd_rule [hoare_triple, hoare_create_case]
+declare length_rule [hoare_triple_direct]
 
 (* Some simple tests *)
 
@@ -79,5 +109,6 @@ theorem "<a \<mapsto>\<^sub>r x> do { a := y; !a } <\<lambda>r. a \<mapsto>\<^su
 theorem "<a \<mapsto>\<^sub>r x> do { a := y; a := z; !a } <\<lambda>r. a \<mapsto>\<^sub>r z * \<up>(r = z)>" by auto2
 theorem "<a \<mapsto>\<^sub>r x> do { y \<leftarrow> !a; ref y} <\<lambda>r. a \<mapsto>\<^sub>r x * r \<mapsto>\<^sub>r x>" by auto2
 theorem "<emp> return x <\<lambda>r. \<up>(r = x)>" by auto2
+theorem "<a \<mapsto>\<^sub>r x * b \<mapsto>\<^sub>r y> comment (a \<mapsto>\<^sub>r x) <\<lambda>r. a \<mapsto>\<^sub>r x * b \<mapsto>\<^sub>r y>" by auto2
 
 end
